%! Tex root: ../master.tex

The quadratic-modified bosonic IKKT model
\begin{equation}
	S_{m}[A_0] = S[A_0] + S_{G}[A_0].
\end{equation}
where
\[
	S[A_0] = - \frac{1}{g_0^2} \mathrm{Tr} [A_0,A_0]^2,\quad
	S_{G}[A_0] = \frac{N_0}{2 v} \mathrm{Tr} A_0^2
.\] 

The partition function
\begin{align*}
	Z[g_0,N_0] = \int \mathrm{e}^{- S_m[A_0]} [\mathrm{d}A_0]
	= \int \mathrm{e}^{-S[A_0] - S_G[A_0]} [\mathrm{d}A_0]\\
	=\int \mathrm{e}^{-S[A]-S_G[A] - S'[\alpha,a;A]-S_G'[\alpha,a]}
	[\mathrm{d}\alpha] [\mathrm{d}\alpha^*][\mathrm{d}a][\mathrm{d}A]
\end{align*}

Assume $Z[g,N]$
\begin{equation}
	Z[g,N] = \int \mathrm{e}^{- S_{\text{eff}}[A'] - S_G[A']} [\mathrm{d}A']
	= Z_0[g_0,N_0]
\end{equation}

\[
	\int  \mathrm{e}^{-S'[\alpha,a;A]-S_G'[\alpha,a]} [\mathrm{d}\alpha]
	[\mathrm{d}\alpha^* ][\mathrm{d}a]
	\sim
	\int (1 - S'[\alpha,a;A]) \mathrm{e}^{-S'_G[\alpha,a]}
	[\mathrm{d}\alpha][\mathrm{d}\alpha^*][\mathrm{d}a]
.\] 
\begin{align*}
	\int (1 - S'[\alpha,a;A]) \mathrm{e}^{-S'_G[\alpha,a]}
	[\mathrm{d}\alpha][\mathrm{d}\alpha^*][\mathrm{d}a]
	\\=
	1 - \frac{2}{g_0^2} \frac{v}{N_0} (D-1) \mathrm{Tr}A^2
	-\frac{2}{g_0^2} \left( \frac{v}{N_0} \right) ^2
	[N^2D^2-ND(2D-1)]
	\\
	\sim \mathrm{e}^{
	 - \frac{2}{g_0^2} \frac{v}{N_0} (D-1) \mathrm{Tr}A^2
	-\frac{2}{g_0^2} \left( \frac{v}{N_0} \right) ^2
	[N^2D^2-ND(2D-1)]
}
\end{align*}

This leads to the following ``action''
\[
	\tilde{S}[A] = S[A] + S_G[A]
	+ \frac{2}{g_0^2} \frac{v}{N_0} (D-1) \mathrm{Tr}A^2
	- \frac{2}{g_0^2} \left( \frac{v}{N_0} \right) ^2[N^2 D^2 - ND(2D-1)]
.\] 

The scaling assumption
\begin{align*}
	N_0 \to N = \lambda N_0 \\
	A_0 \to A' = \lambda^k A\\
	g_0 \to g = \lambda^\gamma g_0
\end{align*}
such that
\[
- \frac{N_0}{2v} \mathrm{Tr}A^2 - \frac{2v}{g_0^2 N_0}(D-1)\mathrm{Tr}A^2
= - \frac{N}{2v} \mathrm{Tr} A'^2
.\] 
\[
	- \frac{1}{g_0^2} \mathrm{Tr}[A,A]^2
	= - \frac{1}{g^2} \mathrm{Tr} [A',A']^2
.\] 

\[
	\lambda^{2k} = \lambda^{-1} \left( 1 + \frac{4v^2(D-1)}{g_0^2 N_0^2} \right) 
	\stackrel{?}{=} \lambda^{-1-\delta}
.\] 
\[
\gamma = 2 k
.\] 
This tells us how the theory changes along the RG flow.

The model will approach the pure IKKT model when $v\to\infty$.
The quadratic term obtained from integrating out blows up.
This invalidates the RG flow interpretation
because a small change in $N$ will result in huge change in $A$.

%%%%%%%%%%%%%%%%%%%%
%  another method  %
%%%%%%%%%%%%%%%%%%%%
The partition function
\[
	Z[g_0,N_0] = \int \mathrm{e}^{-S[A_0]} [\mathrm{d}A_0]
.\] 
Take $a=0$ (experiment, simplicity)
\[
	S[A_0] = S[A] + S'[\alpha;A]
.\] 
\begin{align*}
	S'[\alpha;A] &= - \frac{2}{g_0^2} (\alpha^\mu)^\dagger
	(2 A_\nu A_\mu - A_\mu A_\nu - A^2 \eta_{\mu\nu}) \alpha^\nu \\
				 &- \frac{2}{g_0^2} \left[ (\alpha^\mu)^\dagger \alpha^\nu
	(\alpha_\mu)^\dagger \alpha_\nu - (\alpha^\mu)^\dagger \alpha^\nu
(\alpha_\nu)^\dagger \alpha_\mu - (\alpha^\mu)^\dagger \alpha_\mu
(\alpha^\nu)^\dagger \alpha_\nu\right] 
\end{align*}

Complete the square
\begin{align*}
	 (\alpha^\mu)^\dagger \alpha^\nu
	(\alpha_\mu)^\dagger \alpha_\nu - (\alpha^\mu)^\dagger \alpha^\nu
(\alpha_\nu)^\dagger \alpha_\mu - (\alpha^\mu)^\dagger \alpha_\mu
(\alpha^\nu)^\dagger \alpha_\nu \\
= \frac{1}{1+b^2} \mathrm{Tr} \left[ \alpha^\mu (\alpha^\nu)^\dagger
+ b \alpha^\nu (\alpha^\mu)^\dagger + c \eta^{\mu\nu} \alpha^\rho (\alpha_\rho)^\dagger\right] ^2
\end{align*}
with proper numbers $b,c$.

\begin{gather*}
	\mathrm{Tr}[\alpha^\mu (\alpha^\nu)^\dagger + b \alpha^\nu (\alpha^\mu)^\dagger + c \eta^{\mu\nu} \alpha^\rho (\alpha_{\rho})^\dagger]^2
	\\=
	(1+b^2)(\alpha^\mu)^\dagger \alpha^\nu (\alpha_\mu)^\dagger \alpha_\nu
	+(Dc^2 + 2c + 2bc)(\alpha^\mu)^\dagger \alpha^\nu (\alpha_\nu)^\dagger
	\alpha_\mu + 2b (\alpha^\mu)^\dagger \alpha_\mu (\alpha^\nu)^\dagger \alpha_\nu
\end{gather*}

\begin{align*}
	S'[\alpha;A] &= - \frac{2}{g_0^2} (\alpha^\mu)^\dagger
	(2 A_\nu A_\mu - A_\mu A_\nu - A^2 \eta_{\mu\nu}) \alpha^\nu \\
				 &- \frac{2}{g_0^2(1+b^2)} \mathrm{Tr} \left[ \alpha^\mu (\alpha^\nu)^\dagger
+ b \alpha^\nu (\alpha^\mu)^\dagger + c \eta^{\mu\nu} \alpha^\rho (\alpha_\rho)^\dagger\right] ^2
\end{align*}
Use the ``mean field theory'' to study the second term.
Introduce the auxillary ``field'' $H_{\mu\nu}$
with the action
\[
	S_{\text{aux}} =  \frac{8}{g_0^2(1 + b^2)} \mathrm{Tr} H_{\mu\nu} H^{\mu\nu}
	- \frac{8}{g_0^2(1+b^2)} \mathrm{Tr} H_{\mu\nu}
	\left[ \alpha^\mu (\alpha^\nu)^\dagger + b \alpha^\nu (\alpha^\mu)^\dagger
	+ c \eta^{\mu\nu} \alpha^\rho (\alpha_\rho)^\dagger\right] 
.\] 
Then the following action
\[
	S_{\text{mean}}[H,\alpha;A] = S_{\text{aux}} - \frac{2}{g_0^2} (\alpha^\mu)^\dagger
	(2 A_\nu A_\mu - A_\mu A_\nu - A^2 \eta_{\mu\nu}) \alpha^\nu
\] 
will reproduce the action $S'[\alpha;A]$ after integrating out $H_{\mu\nu}$.
One can write
\[
	S_{\text{mean}}[H,\alpha;A] = \frac{8}{g_0^2 (1+b^2)}
	\mathrm{Tr}H_{\mu\nu}H^{\mu\nu} - \frac{2}{g_0^2}
	(\alpha^\mu)^\dagger M_{\mu\nu} \alpha^\nu
.\] 
with $H\equiv\eta^{\mu\nu}H_{\mu\nu}$
\[
	M_{\mu\nu} = 2A_\nu A_\mu - A_\mu A_\nu - A^2 \eta_{\mu\nu}
	+ \frac{4}{1+b^2} \left( H_{\nu\mu} + b H_{\mu\nu}
	+ c \eta_{\mu\nu}H\right) 
.\] 

\[
	M\equiv\eta^{\mu\nu} M_{\mu\nu} = (1-D)A^2 + \frac{4(1+b+Dc)}{1+b^2}H
.\] 

Integrate out $\alpha,\alpha^\dagger$ to obtain the effective action
\begin{equation*}
	S_{\text{eff}}[H,A] = S[A] + \frac{8}{g_0^2 (1+b^2)} \mathrm{Tr}H_{\mu\nu}H^{\mu\nu}
	- \mathrm{Tr} \ln \left( \frac{2}{g_0^2} M \right) 
\end{equation*}

Note that $H_{\mu\nu},\mu\neq\nu$ is pure Gaussian.
Find the saddle point equation for $H_{11},H_{22},\cdots$.
$H_{\mu\nu}$ is matrix? or number $H_{\mu\nu}\mathds{1}$.
